thy/Iptables_Semantics/Examples/Small_Examples.thy
@@ -1,0 +1,85 @@
+theory Small_Examples
+imports "../Primitive_Matchers/Code_Interface"
+begin
+
+section\<open>Small Examples\<close>
+context
+begin
+  lemma "let fw = [''FORWARD'' \<mapsto> [Rule (Match (Src (IpAddrNetmask (ipv4addr_of_dotdecimal (10,0,0,0)) 8))) (Call ''foo'')],
+                   ''foo'' \<mapsto> [Rule (Match (Src (IpAddrNetmask (ipv4addr_of_dotdecimal (10,128,0,0)) 9))) action.Return,
+                               Rule (Match (Prot (Proto TCP))) action.Accept]
+                   ] in
+    let simplfw = to_simple_firewall
+      (upper_closure (optimize_matches abstract_for_simple_firewall
+        (upper_closure (packet_assume_new (unfold_ruleset_FORWARD action.Drop fw)))))
+    in map simple_rule_ipv4_toString simplfw =
+    [''ACCEPT     tcp  --  10.0.0.0/9            0.0.0.0/0    '',
+     ''DROP     all  --  0.0.0.0/0            0.0.0.0/0    '']" by eval
+  
+  private definition "cool_example \<equiv> (let fw = 
+                [''FORWARD'' \<mapsto> [Rule (Match (Src (IpAddrNetmask (ipv4addr_of_dotdecimal (10,0,0,0)) 8))) (Call ''foo'')],
+                 ''foo'' \<mapsto> [Rule (MatchNot (Match (Src (IpAddrNetmask (ipv4addr_of_dotdecimal (10,0,0,0)) 9)))) action.Drop,
+                             Rule (Match (Prot (Proto TCP))) action.Accept]
+                 ] in
+    to_simple_firewall (upper_closure (optimize_matches abstract_for_simple_firewall
+                          (upper_closure (packet_assume_new (unfold_ruleset_FORWARD action.Drop fw))))))"
+  lemma " map simple_rule_ipv4_toString cool_example =
+    [''DROP     all  --  10.128.0.0/9            0.0.0.0/0    '',
+     ''ACCEPT     tcp  --  10.0.0.0/8            0.0.0.0/0    '',
+     ''DROP     all  --  0.0.0.0/0            0.0.0.0/0    '']"
+  by eval
+  
+  lemma "map ipv4addr_wordinterval_toString (getParts cool_example) =
+    [''{10.128.0.0 .. 10.255.255.255}'',
+     ''{10.0.0.0 .. 10.127.255.255}'',
+     ''{0.0.0.0 .. 9.255.255.255} u {11.0.0.0 .. 255.255.255.255}'']" by eval
+  
+  lemma "map ipv4addr_wordinterval_toString (build_ip_partition parts_connection_ssh cool_example) =
+    [''{0.0.0.0 .. 9.255.255.255} u {10.128.0.0 .. 255.255.255.255}'',
+     ''{10.0.0.0 .. 10.127.255.255}'']" by eval
+  
+  (*it is not minimal if we allow to further compress the node definitions?
+  the receiver nodes could be combined to UNIV
+  But minimal for a symmetric matrix*)
+  lemma "access_matrix_pretty_ipv4 parts_connection_ssh cool_example =
+    ([(''0.0.0.0'', ''{0.0.0.0 .. 9.255.255.255} u {10.128.0.0 .. 255.255.255.255}''),
+      (''10.0.0.0'', ''{10.0.0.0 .. 10.127.255.255}'')],
+     [(''10.0.0.0'', ''0.0.0.0''),
+      (''10.0.0.0'', ''10.0.0.0'')])" by eval
+end
+context
+begin
+  (*now with a destination IP*)
+  private definition "cool_example2 \<equiv> (let fw =
+    [''FORWARD'' \<mapsto> [Rule (Match (Src (IpAddrNetmask (ipv4addr_of_dotdecimal (10,0,0,0)) 8))) (Call ''foo'')],
+     ''foo'' \<mapsto> [Rule (MatchNot (Match (Src (IpAddrNetmask (ipv4addr_of_dotdecimal (10,0,0,0)) 9)))) action.Drop,
+                 Rule (MatchAnd (Match (Prot (Proto TCP))) (Match (Dst (IpAddrNetmask (ipv4addr_of_dotdecimal (10,0,0,42)) 32)))) action.Accept]
+                ] in
+    to_simple_firewall (upper_closure (optimize_matches abstract_for_simple_firewall
+                          (upper_closure (packet_assume_new (unfold_ruleset_FORWARD action.Drop fw))))))"
+  lemma "map simple_rule_ipv4_toString cool_example2 =
+    [''DROP     all  --  10.128.0.0/9            0.0.0.0/0    '',
+     ''ACCEPT     tcp  --  10.0.0.0/8            10.0.0.42/32    '',
+     ''DROP     all  --  0.0.0.0/0            0.0.0.0/0    '']" by eval
+  
+  (*not minimal*)
+  lemma "map ipv4addr_wordinterval_toString (getParts cool_example2) =
+    [''{10.128.0.0 .. 10.255.255.255}'', ''10.0.0.42'',
+     ''{10.0.0.0 .. 10.0.0.41} u {10.0.0.43 .. 10.127.255.255}'',
+     ''{0.0.0.0 .. 9.255.255.255} u {11.0.0.0 .. 255.255.255.255}'']" by eval
+  
+  lemma "map ipv4addr_wordinterval_toString (build_ip_partition parts_connection_ssh cool_example2) =
+    [''{0.0.0.0 .. 9.255.255.255} u {10.128.0.0 .. 255.255.255.255}'', ''10.0.0.42'',
+     ''{10.0.0.0 .. 10.0.0.41} u {10.0.0.43 .. 10.127.255.255}'']" by eval
+  
+  lemma "access_matrix_pretty_ipv4 parts_connection_ssh cool_example2 =
+    ([(''0.0.0.0'', ''{0.0.0.0 .. 9.255.255.255} u {10.128.0.0 .. 255.255.255.255}''),
+      (''10.0.0.42'', ''10.0.0.42''),
+      (''10.0.0.0'', ''{10.0.0.0 .. 10.0.0.41} u {10.0.0.43 .. 10.127.255.255}'')
+     ],
+     [(''10.0.0.42'', ''10.0.0.42''),
+      (''10.0.0.0'', ''10.0.0.42'')
+     ])" by eval
+  end
+
+end
